Abbreviation for one, more automatizations, remove duplicate name (GenExtD).

src/Choice_Axiom.thy
@@ -125,102 +125,92 @@ proof (intro CollectI ballI)
     "\<exists>x\<in>\<alpha>. induced_surj(f, a, e) ` x = y" by auto
 qed
 
+definition
+  upair_name' :: "i \<Rightarrow> i \<Rightarrow> i \<Rightarrow> i" where
+  "upair_name'(\<tau>,\<rho>,on) \<equiv> Upair(\<langle>\<tau>,on\<rangle>,\<langle>\<rho>,on\<rangle>)"
+
+relativize "upair_name'" "is_upair_name"
+synthesize "upair_name" from_definition "is_upair_name" 
+definition
+  opair_name' :: "i \<Rightarrow> i \<Rightarrow> i \<Rightarrow> i" where
+  "opair_name'(\<tau>,\<rho>,on) \<equiv> upair_name'(upair_name'(\<tau>,\<tau>,on),upair_name'(\<tau>,\<rho>,on),on)"
+
+relativize "opair_name'" "is_opair_name"
+synthesize "opair_name" from_definition "is_opair_name"
+
 context G_generic
 begin
 
-definition
-  upair_name :: "i \<Rightarrow> i \<Rightarrow> i" where
-  "upair_name(\<tau>,\<rho>) \<equiv> Upair(\<langle>\<tau>,one\<rangle>,\<langle>\<rho>,one\<rangle>)"
+abbreviation upair_name where
+  "upair_name(\<tau>,\<rho>) \<equiv> upair_name'(\<tau>,\<rho>,\<one>)"
+
+abbreviation opair_name where
+  "opair_name(\<tau>,\<rho>) \<equiv> opair_name'(\<tau>,\<rho>,\<one>)"
 
 lemma Upair_simp : "Upair(a,b) = {a,b}"
   by auto
 
-relativize "upair_name" "is_upair_name"
-
 lemma upair_name_abs :
   assumes "x\<in>M" "y\<in>M" "z\<in>M"
-  shows "is_upair_name(##M,x,y,z) \<longleftrightarrow> z = upair_name(x,y)"
-  unfolding is_upair_name_def upair_name_def
+  shows "is_upair_name(##M,x,y,\<one>,z) \<longleftrightarrow> z = upair_name(x,y)"
+  unfolding is_upair_name_def upair_name'_def
   using assms zero_in_M one_in_M  empty_abs pair_abs pair_in_M_iff upair_in_M_iff upair_abs
   Upair_simp
   by simp
 
-definition
-  opair_name :: "i \<Rightarrow> i \<Rightarrow> i" where
-  "opair_name(\<tau>,\<rho>) \<equiv> upair_name(upair_name(\<tau>,\<tau>),upair_name(\<tau>,\<rho>))"
-
-relativize "opair_name" "is_opair_name"
-
 lemma upair_name_closed :
   "\<lbrakk> x\<in>M; y\<in>M \<rbrakk> \<Longrightarrow> upair_name(x,y)\<in>M"
-  unfolding upair_name_def using upair_in_M_iff pair_in_M_iff one_in_M upair_in_M_iff Upair_simp
+  unfolding upair_name'_def using upair_in_M_iff pair_in_M_iff one_in_M upair_in_M_iff Upair_simp
   by simp
 
-definition
-  upair_name_fm :: "[i,i,i,i] \<Rightarrow> i" where
-  "upair_name_fm(x,y,o,z) \<equiv> Exists(Exists(And(pair_fm(x#+2,o#+2,1),
-                                          And(pair_fm(y#+2,o#+2,0),upair_fm(1,0,z#+2)))))"
-
-lemma upair_name_fm_type[TC] :
-    "\<lbrakk> s\<in>nat;x\<in>nat;y\<in>nat;o\<in>nat\<rbrakk> \<Longrightarrow> upair_name_fm(s,x,y,o)\<in>formula"
-  unfolding upair_name_fm_def by simp
-
-lemma sats_upair_name_fm :
-  assumes "x\<in>nat" "y\<in>nat" "z\<in>nat" "o\<in>nat" "env\<in>list(M)""nth(o,env)=one"
+lemma sats_upair_name_fm' :
+  assumes "x\<in>nat" "y\<in>nat" "z\<in>nat" "o\<in>nat" "env\<in>list(M)""nth(o,env)=\<one>"
   shows
-    "sats(M,upair_name_fm(x,y,o,z),env) \<longleftrightarrow> is_upair_name(##M,nth(x,env),nth(y,env),nth(z,env))"
+    "sats(M,upair_name_fm(x,y,o,z),env) \<longleftrightarrow> is_upair_name(##M,nth(x,env),nth(y,env),nth(o,env),nth(z,env))"
   unfolding upair_name_fm_def is_upair_name_def
-  using assms zero_in_M  empty_abs pair_abs one_in_M pair_in_M_iff Upair_simp upair_in_M_iff
+  using assms sats_upair_name_fm
   by auto
 
 lemma opair_name_abs :
   assumes "x\<in>M" "y\<in>M" "z\<in>M"
-  shows "is_opair_name(##M,x,y,z) \<longleftrightarrow> z = opair_name(x,y)"
-  unfolding is_opair_name_def opair_name_def using assms upair_name_abs upair_name_closed by simp
+  shows "is_opair_name(##M,x,y,\<one>,z) \<longleftrightarrow> z = opair_name(x,y)"
+  unfolding is_opair_name_def opair_name'_def 
+  using assms upair_name_abs upair_name_closed by simp
 
 lemma opair_name_closed :
   "\<lbrakk> x\<in>M; y\<in>M \<rbrakk> \<Longrightarrow> opair_name(x,y)\<in>M"
-  unfolding opair_name_def using upair_name_closed by simp
-
-definition
-  opair_name_fm :: "[i,i,i,i] \<Rightarrow> i" where
-  "opair_name_fm(x,y,o,z) \<equiv> Exists(Exists(And(upair_name_fm(x#+2,x#+2,o#+2,1),
-                    And(upair_name_fm(x#+2,y#+2,o#+2,0),upair_name_fm(1,0,o#+2,z#+2)))))"
-
-lemma opair_name_fm_type[TC] :
-    "\<lbrakk> s\<in>nat;x\<in>nat;y\<in>nat;o\<in>nat\<rbrakk> \<Longrightarrow> opair_name_fm(s,x,y,o)\<in>formula"
-  unfolding opair_name_fm_def by simp
+  unfolding opair_name'_def 
+  using upair_name_closed by simp
 
 lemma sats_opair_name_fm :
-  assumes "x\<in>nat" "y\<in>nat" "z\<in>nat" "o\<in>nat" "env\<in>list(M)""nth(o,env)=one"
+  assumes "x\<in>nat" "y\<in>nat" "z\<in>nat" "o\<in>nat" "env\<in>list(M)" "nth(o,env)=\<one>"
   shows
-    "sats(M,opair_name_fm(x,y,o,z),env) \<longleftrightarrow> is_opair_name(##M,nth(x,env),nth(y,env),nth(z,env))"
-  unfolding opair_name_fm_def is_opair_name_def
-  using assms sats_upair_name_fm
+    "sats(M,opair_name_fm(x,y,o,z),env) \<longleftrightarrow> is_opair_name(##M,nth(x,env),nth(y,env),nth(o,env),nth(z,env))"
+  using assms sats_opair_name_fm
   by auto
 
 lemma val_upair_name : "val(P,G,upair_name(\<tau>,\<rho>)) = {val(P,G,\<tau>),val(P,G,\<rho>)}"
-  unfolding upair_name_def using val_Upair Upair_simp generic one_in_G one_in_P by simp
+  unfolding upair_name'_def using val_Upair Upair_simp generic one_in_G one_in_P by simp
 
 lemma val_opair_name : "val(P,G,opair_name(\<tau>,\<rho>)) = \<langle>val(P,G,\<tau>),val(P,G,\<rho>)\<rangle>"
-  unfolding opair_name_def Pair_def using val_upair_name by simp
+  unfolding opair_name'_def Pair_def using val_upair_name by simp
 
-lemma val_RepFun_one: "val(P,G,{\<langle>f(x),one\<rangle> . x\<in>a}) = {val(P,G,f(x)) . x\<in>a}"
+lemma val_RepFun_one: "val(P,G,{\<langle>f(x),\<one>\<rangle> . x\<in>a}) = {val(P,G,f(x)) . x\<in>a}"
 proof -
   let ?A = "{f(x) . x \<in> a}"
-  let ?Q = "\<lambda>\<langle>x,p\<rangle> . p = one"
-  have "one \<in> P\<inter>G" using generic one_in_G one_in_P by simp
-  have "{\<langle>f(x),one\<rangle> . x \<in> a} = {t \<in> ?A \<times> P . ?Q(t)}"
+  let ?Q = "\<lambda>\<langle>x,p\<rangle> . p = \<one>"
+  have "\<one> \<in> P\<inter>G" using generic one_in_G one_in_P by simp
+  have "{\<langle>f(x),\<one>\<rangle> . x \<in> a} = {t \<in> ?A \<times> P . ?Q(t)}"
     using one_in_P by force
   then
-  have "val(P,G,{\<langle>f(x),one\<rangle>  . x \<in> a}) = val(P,G,{t \<in> ?A \<times> P . ?Q(t)})"
+  have "val(P,G,{\<langle>f(x),\<one>\<rangle>  . x \<in> a}) = val(P,G,{t \<in> ?A \<times> P . ?Q(t)})"
     by simp
   also
   have "... = {val(P,G,t) .. t \<in> ?A , \<exists>p\<in>P\<inter>G . ?Q(\<langle>t,p\<rangle>)}"
     using val_of_name_alt by simp
   also
   have "... = {val(P,G,t) . t \<in> ?A }"
-    using \<open>one\<in>P\<inter>G\<close> by force
+    using \<open>\<one>\<in>P\<inter>G\<close> by force
   also
   have "... = {val(P,G,f(x)) . x \<in> a}"
     by auto
@@ -235,30 +225,30 @@ interpretation mgzf: M_ZF_trans "M[G]"
     strong_replacement_in_MG separation_in_MG infinity_in_MG
   by unfold_locales simp_all
 
-(* y = opair_name(check(\<beta>),s`\<beta>) *)
-(*relativize_tm "opair_name(x,s`x)" "is_opname_check"*)
+(* FIXME: we could have this synthesized if is_check were parameterised by the class. 
+*)
 definition
   is_opname_check :: "[i,i,i] \<Rightarrow> o" where
   "is_opname_check(s,x,y) \<equiv> \<exists>chx\<in>M. \<exists>sx\<in>M. is_check(x,chx) \<and> fun_apply(##M,s,x,sx) \<and>
-                             is_opair_name(##M,chx,sx,y)"
+                             is_opair_name(##M,chx,sx,\<one>,y)"
 
 definition
   opname_check_fm :: "[i,i,i,i] \<Rightarrow> i" where
-  "opname_check_fm(s,x,y,o) \<equiv> Exists(Exists(And(check_fm(2#+x,2#+o,1),
+  "opname_check_fm(o,s,x,y) \<equiv> Exists(Exists(And(check_fm(2#+x,2#+o,1),
                               And(fun_apply_fm(2#+s,2#+x,0),opair_name_fm(1,0,2#+o,2#+y)))))"
 
 lemma opname_check_fm_type[TC] :
-  "\<lbrakk> s\<in>nat;x\<in>nat;y\<in>nat;o\<in>nat\<rbrakk> \<Longrightarrow> opname_check_fm(s,x,y,o)\<in>formula"
+  "\<lbrakk> s\<in>nat;x\<in>nat;y\<in>nat;o\<in>nat\<rbrakk> \<Longrightarrow> opname_check_fm(o,s,x,y)\<in>formula"
   unfolding opname_check_fm_def by simp
 
 lemma sats_opname_check_fm:
-  assumes "x\<in>nat" "y\<in>nat" "z\<in>nat" "o\<in>nat" "env\<in>list(M)" "nth(o,env)=one"
+  assumes "x\<in>nat" "y\<in>nat" "z\<in>nat" "o\<in>nat" "env\<in>list(M)" "nth(o,env)=\<one>"
           "y<length(env)"
   shows
-    "sats(M,opname_check_fm(x,y,z,o),env) \<longleftrightarrow> is_opname_check(nth(x,env),nth(y,env),nth(z,env))"
+    "sats(M,opname_check_fm(o,x,y,z),env) \<longleftrightarrow> is_opname_check(nth(x,env),nth(y,env),nth(z,env))"
   unfolding opname_check_fm_def is_opname_check_def
-  using assms sats_check_fm sats_opair_name_fm one_in_M by simp
-
+  using assms sats_check_fm sats_opair_name_fm one_in_M 
+  by simp
 
 lemma opname_check_abs :
   assumes "s\<in>M" "x\<in>M" "y\<in>M"
@@ -272,19 +262,20 @@ lemma repl_opname_check :
   shows
    "{opair_name(check(x),f`x). x\<in>A}\<in>M"
 proof -
-  have "arity(opname_check_fm(3,0,1,2))= 4"
-    unfolding fm_definitions opname_check_fm_def opair_name_fm_def upair_name_fm_def
+  have "arity(opname_check_fm(3,2,0,1))= 4"
+    unfolding fm_definitions opname_check_fm_def
     by (simp add:ord_simp_union arity)
   moreover
   have "x\<in>A \<Longrightarrow> opair_name(check(x), f ` x)\<in>M" for x
     using assms opair_name_closed apply_closed transitivity check_in_M
     by simp
   ultimately
-  show ?thesis using assms opname_check_abs[of f] sats_opname_check_fm
+  show ?thesis 
+    using assms opname_check_abs[of f] sats_opname_check_fm
         one_in_M transitivity
-        Replace_relativized_in_M[of "opname_check_fm(3,0,1,2)" "[one,f]" _ "is_opname_check(f)"
+    Replace_relativized_in_M[of "opname_check_fm(3,2,0,1)" "[f,\<one>]" A "is_opname_check(f)"
                     "\<lambda>x. opair_name(check(x),f`x)"]
-    by auto
+    by simp
 qed
 
 theorem choice_in_MG:
@@ -309,12 +300,12 @@ proof -
     let ?A="domain(\<tau>)\<times>P"
     let ?g = "{opair_name(check(\<beta>),s`\<beta>). \<beta>\<in>\<alpha>}"
     have "?g \<in> M" using \<open>s\<in>M\<close> \<open>\<alpha>\<in>M\<close> repl_opname_check by simp
-    let ?f_dot="{\<langle>opair_name(check(\<beta>),s`\<beta>),one\<rangle>. \<beta>\<in>\<alpha>}"
-    have "?f_dot = ?g \<times> {one}" by blast
-    from one_in_M have "{one} \<in> M" using singleton_closed by simp
+    let ?f_dot="{\<langle>opair_name(check(\<beta>),s`\<beta>),\<one>\<rangle>. \<beta>\<in>\<alpha>}"
+    have "?f_dot = ?g \<times> {\<one>}" by blast
+    from one_in_M have "{\<one>} \<in> M" using singleton_closed by simp
     define f where
       "f \<equiv> val(P,G,?f_dot)"
-    from \<open>{one}\<in>M\<close> \<open>?g\<in>M\<close> \<open>?f_dot = ?g\<times>{one}\<close>
+    from \<open>{\<one>}\<in>M\<close> \<open>?g\<in>M\<close> \<open>?f_dot = ?g\<times>{\<one>}\<close>
     have "?f_dot\<in>M"
       using cartprod_closed by simp
     then
