src/Cardinal_Preservation.thy
@@ -289,7 +289,7 @@ definition check_fm' where
 
 lemma ccc_fun_closed_lemma_aux:
   assumes "f_dot\<in>M" "p\<in>M" "a\<in>M" "b\<in>M"
-  shows "{q \<in> P . q \<preceq> p \<and> (M, [q, P, leq, one, f_dot, a\<^sup>v, b\<^sup>v] \<Turnstile> forces(\<cdot>0`1 is 2\<cdot> ))} \<in> M"
+  shows "{q \<in> P . q \<preceq> p \<and> (M, [q, P, leq, \<one>, f_dot, a\<^sup>v, b\<^sup>v] \<Turnstile> forces(\<cdot>0`1 is 2\<cdot> ))} \<in> M"
 proof -
   have "\<cdot>0`1 is 2\<cdot> \<in> formula" "arity(\<cdot>0`1 is 2\<cdot> ) = 3"
     using arity_fun_apply_fm union_abs1
@@ -306,9 +306,9 @@ qed
 
 lemma ccc_fun_closed_lemma_aux2:
   assumes "B\<in>M" "f_dot\<in>M" "p\<in>M" "a\<in>M"
-  shows "(##M)(\<lambda>b\<in>B. {q \<in> P . q \<preceq> p \<and> (M, [q, P, leq, one, f_dot, a\<^sup>v, b\<^sup>v] \<Turnstile> forces(\<cdot>0`1 is 2\<cdot> ))})"
+  shows "(##M)(\<lambda>b\<in>B. {q \<in> P . q \<preceq> p \<and> (M, [q, P, leq, \<one>, f_dot, a\<^sup>v, b\<^sup>v] \<Turnstile> forces(\<cdot>0`1 is 2\<cdot> ))})"
 proof -
-  have "separation(##M, \<lambda>z. M, [snd(z), P, leq, one, f_dot, \<tau>, fst(fst(z))\<^sup>v] \<Turnstile> forces(\<cdot>0`1 is 2\<cdot> ))"
+  have "separation(##M, \<lambda>z. M, [snd(z), P, leq, \<one>, f_dot, \<tau>, fst(fst(z))\<^sup>v] \<Turnstile> forces(\<cdot>0`1 is 2\<cdot> ))"
     if "\<tau>\<in>M" for \<tau>
   proof -
     let ?f_fm="snd_fm(1,0)"
@@ -345,7 +345,7 @@ lemma ccc_fun_closed_lemma:
   assumes "A\<in>M" "B\<in>M" "f_dot\<in>M" "p\<in>M"
   shows "(\<lambda>a\<in>A. {b\<in>B. \<exists>q\<in>P. q \<preceq> p \<and> (q \<tturnstile> \<cdot>0`1 is 2\<cdot> [f_dot, a\<^sup>v, b\<^sup>v])}) \<in> M"
 proof -
-  have "separation(##M, \<lambda>z. M, [snd(z), P, leq, one, f_dot, fst(fst(fst(z)))\<^sup>v, snd(fst(z))\<^sup>v] \<Turnstile> forces(\<cdot>0`1 is 2\<cdot> ))"
+  have "separation(##M, \<lambda>z. M, [snd(z), P, leq, \<one>, f_dot, fst(fst(fst(z)))\<^sup>v, snd(fst(z))\<^sup>v] \<Turnstile> forces(\<cdot>0`1 is 2\<cdot> ))"
   proof -
     note types = assms leq_in_M P_in_M one_in_M
     let ?f_fm="snd_fm(1,0)"
@@ -368,7 +368,7 @@ proof -
       by simp
   qed
   moreover
-  have  "separation(##M, \<lambda>z. M, [snd(z), P, leq, one, f_dot, \<tau>, fst(z)\<^sup>v] \<Turnstile> forces(\<cdot>0`1 is 2\<cdot> ))"
+  have  "separation(##M, \<lambda>z. M, [snd(z), P, leq, \<one>, f_dot, \<tau>, fst(z)\<^sup>v] \<Turnstile> forces(\<cdot>0`1 is 2\<cdot> ))"
     if "\<tau>\<in>M" for \<tau>
   proof -
     let ?f_fm="snd_fm(1,0)"
@@ -463,7 +463,7 @@ proof -
       using ccc_fun_closed_lemma_aux[OF \<open>f_dot\<in>M\<close> \<open>p\<in>M\<close> \<open>a\<in>M\<close> 2] transitivity[of _ "F`a"]
       by simp
     moreover
-    have 4:"lam_replacement(##M,\<lambda>b. {q \<in> P . q \<preceq> p \<and> (M, [q, P, leq, one, f_dot, a\<^sup>v, b\<^sup>v] \<Turnstile> forces(\<cdot>0`1 is 2\<cdot> ))})"
+    have 4:"lam_replacement(##M,\<lambda>b. {q \<in> P . q \<preceq> p \<and> (M, [q, P, leq, \<one>, f_dot, a\<^sup>v, b\<^sup>v] \<Turnstile> forces(\<cdot>0`1 is 2\<cdot> ))})"
       using ccc_fun_closed_lemma_aux2[OF _ \<open>f_dot\<in>M\<close> \<open>p\<in>M\<close> \<open>a\<in>M\<close>]
         lam_replacement_iff_lam_closed[THEN iffD2]
         ccc_fun_closed_lemma_aux[OF  \<open>f_dot\<in>M\<close> \<open>p\<in>M\<close> \<open>a\<in>M\<close>]
