src/Internal_ZFC_Axioms.thy
@@ -270,7 +270,7 @@ schematic_goal sats_univalent_fm_auto:
   assumes 
     (*    Q_iff_sats:"\<And>a b z env aa bb. nth(a,Cons(z,env)) = aa \<Longrightarrow> nth(b,Cons(z,env)) = bb \<Longrightarrow> z\<in>A 
           \<Longrightarrow> aa \<in> A \<Longrightarrow> bb \<in> A \<Longrightarrow> env\<in> list(A) \<Longrightarrow> 
-                 Q(aa,bb) \<longleftrightarrow> (A, Cons(z,env) \<Turnstile> (Q_fm(a,b)))" \<comment> \<open>using only one formula\<close> *)
+                 Q(aa,bb) \<longleftrightarrow> (A, Cons(z,env) \<Turnstile> (Q_fm(a,b)))" \<comment> \<open>using only \<one> formula\<close> *)
     Q_iff_sats:"\<And>x y z. x \<in> A \<Longrightarrow> y \<in> A \<Longrightarrow> z\<in>A \<Longrightarrow> 
                  Q(x,z) \<longleftrightarrow> (A,Cons(z,Cons(y,Cons(x,env))) \<Turnstile> Q1_fm)"
        "\<And>x y z. x \<in> A \<Longrightarrow> y \<in> A \<Longrightarrow> z\<in>A \<Longrightarrow> 
